trans2Nt existence

Stimpfle/CNF.thy
@@ -34,28 +34,28 @@ lemma upgr_noeProds:
 
 (* Chomsky Normal Form *)
 
-definition trans1Tmnl :: "'n \<Rightarrow> 't \<Rightarrow> ('n, 't) prods \<Rightarrow> ('n, 't) prods \<Rightarrow> bool" where 
-      "trans1Tmnl A t P P' \<equiv> (
+definition trans1Tm :: "'n::infinite \<Rightarrow> 't \<Rightarrow> ('n, 't) prods \<Rightarrow> ('n, 't) prods \<Rightarrow> bool" where 
+      "trans1Tm A t P P' \<equiv> (
     \<exists> l r p s. (l,r) \<in> set P \<and> (r = p@[Tm t]@s) 
-    \<and> (p \<noteq> [] \<or> s \<noteq> []) \<and> (A \<notin> nts (set P))
+    \<and> (p \<noteq> [] \<or> s \<noteq> []) \<and> (A = fresh P)
     \<and> (P' = ((removeAll (l,r) P) @ [(A,[Tm t]), (l, p@[Nt A]@s)])))"
 
-lemma trans1Tmnl_noeProds:
+lemma trans1Tm_noeProds:
   assumes "noeProds (set P)"
-    and "trans1Tmnl A t P P'"
+    and "trans1Tm A t P P'"
   shows "noeProds (set P')"
-  using assms unfolding trans1Tmnl_def noeProds_def by force
+  using assms unfolding trans1Tm_def noeProds_def by force
 
-lemma trans1Tmnl_noUnitProds:
+lemma trans1Tm_noUnitProds:
   assumes "noUnitProds (set P)"
-    and "trans1Tmnl A t P P'"
+    and "trans1Tm A t P P'"
   shows "noUnitProds (set P')"
 proof -
   have 1: "(\<nexists>l A. (l,[Nt A]) \<in> (set P))"
     using assms(1) unfolding noUnitProds_def by simp
   obtain l r p s where "(l,r) \<in> set P \<and> (r = p@[Tm t]@s) \<and> (p \<noteq> [] \<or> s \<noteq> []) 
       \<and> set P' = ((set P - {(l,r)}) \<union> {(A,[Tm t]), (l, p@[Nt A]@s)})" (is "?lrps")
-    using assms(2) set_removeAll unfolding trans1Tmnl_def by force
+    using assms(2) set_removeAll unfolding trans1Tm_def by force
   hence "\<nexists>l' A'. (l,[Nt A']) \<in> {(A,[Tm t]), (l, p@[Nt A]@s)}" 
     using Cons_eq_append_conv by fastforce
   hence "\<nexists>l' A'. (l',[Nt A']) \<in> ((set P - {(l,r)}) \<union> {(A,[Tm t]), (l, p@[Nt A]@s)})"
@@ -77,29 +77,23 @@ fun badTmsCount :: "('n,'t) prods \<Rightarrow> nat" where
   "badTmsCount [] = 0" |
   "badTmsCount (p#ps) = (prodTms p) + badTmsCount ps"
 
-(* My definition based on sets instead of list iteration *)
-definition badTms :: "('n,'t) prodS \<Rightarrow> bool" where
-  "badTms P = (\<forall>p \<in> P. prodTms p = 0)"
-
-find_consts "'a set \<Rightarrow> nat"
-
-lemma badTms_eq_badTmsCount: "badTms (set P) \<longleftrightarrow> badTmsCount P = 0"
- unfolding badTms_def apply (induction P) by auto
+lemma badTmsCountSet: "(\<forall>p \<in> set P. prodTms p = 0) \<longleftrightarrow> badTmsCount P = 0"
+ apply (induction P) by auto
 
 fun badNtsCount :: "('n,'t) prods \<Rightarrow> nat" where
   "badNtsCount [] = 0" |
   "badNtsCount (p#ps) = (prodNts p) + badNtsCount ps"
 
-definition badNts :: "('n,'t) prodS \<Rightarrow> bool" where
-  "badNts P = (\<forall>p \<in> P. prodNts p = 0)"
+lemma badNtsCountSet: "(\<forall>p \<in> set P. prodNts p = 0) \<longleftrightarrow> badNtsCount P = 0"
+ apply (induction P) by auto
 
 definition cnf :: "('n,'t) prods \<Rightarrow> bool" where
   "cnf P = ((badTmsCount P = 0) \<and> (badNtsCount P = 0))"
 
-definition trans2Nt :: "'n \<Rightarrow> 'n \<Rightarrow> 'n \<Rightarrow> ('n,'t) prods \<Rightarrow> ('n,'t) prods \<Rightarrow> bool" where
+definition trans2Nt :: "'n::infinite \<Rightarrow> 'n \<Rightarrow> 'n \<Rightarrow> ('n,'t) prods \<Rightarrow> ('n,'t) prods \<Rightarrow> bool" where
       "trans2Nt A B\<^sub>1 B\<^sub>2 P P' \<equiv> (
     \<exists>l r p s. (l,r) \<in> set P \<and> (r = p@[Nt B\<^sub>1,Nt B\<^sub>2]@s)
-    \<and> (p \<noteq> [] \<or> s \<noteq> []) \<and> (A \<notin> nts (set P))
+    \<and> (p \<noteq> [] \<or> s \<noteq> []) \<and> (A = fresh P)
     \<and> (P' = ((removeAll (l,r) P) @ [(A, [Nt B\<^sub>1,Nt B\<^sub>2]), (l, p@[Nt A]@s)])))"
 
 lemma trans2Nt_noeProds:
@@ -130,11 +124,11 @@ qed
 lemma trans2Nt_aux1:
   assumes "trans2Nt A B\<^sub>1 B\<^sub>2 P P'"
   shows "A \<noteq> B\<^sub>1 \<and> A \<noteq> B\<^sub>2"
-  using assms unfolding trans2Nt_def nts_def by auto
+  using assms fresh unfolding trans2Nt_def nts_def by fastforce
 
 
 lemma cnf_r1Tm: 
-  assumes "trans1Tmnl A t P P'"
+  assumes "trans1Tm A t P P'"
     and "set P \<turnstile> lhs \<Rightarrow> rhs"
   shows "set P' \<turnstile> lhs \<Rightarrow>* rhs"
 proof -
@@ -142,7 +136,7 @@ proof -
     using assms(2) derive.cases by meson
   obtain l r p s where "(l,r) \<in> set P \<and> (r = p@[Tm t]@s) \<and> (p \<noteq> [] \<or> s \<noteq> []) \<and> (A \<notin> nts (set P))
       \<and> set P' = ((set P - {(l,r)}) \<union> {(A,[Tm t]), (l, p@[Nt A]@s)})" (is "?lrps")
-    using assms(1) set_removeAll unfolding trans1Tmnl_def by force
+    using assms(1) set_removeAll fresh unfolding trans1Tm_def by fastforce
   thus ?thesis 
   proof (cases "u = l")
     case True
@@ -178,7 +172,7 @@ proof -
     using assms(2) derive.cases by meson
   obtain l r p s where "(l,r) \<in> set P \<and> (r = p@[Nt B\<^sub>1,Nt B\<^sub>2]@s) \<and> (p \<noteq> [] \<or> s \<noteq> []) \<and> (A \<notin> nts (set P))
     \<and> (set P' = ((set P - {(l,r)}) \<union> {(A, [Nt B\<^sub>1,Nt B\<^sub>2]), (l, p@[Nt A]@s)}))" (is "?lrps")
-    using assms(1) set_removeAll unfolding trans2Nt_def by force
+    using assms(1) set_removeAll fresh unfolding trans2Nt_def by fastforce
   thus ?thesis
   proof (cases "u = l")
     case True
@@ -215,16 +209,16 @@ definition noNewNts :: "('n, 't) prods \<Rightarrow> ('n, 't) sym set \<Rightarr
   "noNewNts P rhS = (\<forall>r. (Nt r \<in> rhS) \<longrightarrow> r \<in> nts (set P))"
 
 lemma slemma1_1: 
-  assumes "trans1Tmnl A t P P'"
+  assumes "trans1Tm A t P P'"
     and "(A, \<alpha>) \<in> set P'"
   shows "\<alpha> = [Tm t]"
 proof -
   have "A \<notin> nts (set P)"
-    using assms(1) unfolding trans1Tmnl_def by blast
+    using assms(1) fresh unfolding trans1Tm_def by blast
   hence "\<nexists>\<alpha>. (A, \<alpha>) \<in> set P"
     unfolding nts_def by auto
   hence "\<nexists>\<alpha>. \<alpha> \<noteq> [Tm t] \<and> (A, \<alpha>) \<in> set P'"
-    using assms(1) unfolding trans1Tmnl_def by auto
+    using assms(1) unfolding trans1Tm_def by auto
   thus ?thesis 
     using assms(2) by blast
 qed
@@ -235,7 +229,7 @@ lemma slemma1_1Nt:
   shows "\<alpha> = [Nt B\<^sub>1,Nt B\<^sub>2]"
 proof -
   have "A \<notin> nts (set P)"
-    using assms(1) unfolding trans2Nt_def by blast
+    using assms(1) fresh unfolding trans2Nt_def by blast
   hence "\<nexists>\<alpha>. (A, \<alpha>) \<in> set P"
     unfolding nts_def  by auto
   hence "\<nexists>\<alpha>. \<alpha> \<noteq> [Nt B\<^sub>1,Nt B\<^sub>2] \<and> (A, \<alpha>) \<in> set P'"
@@ -270,12 +264,12 @@ lemma nts_correct: "A \<notin> nts P \<Longrightarrow> (\<nexists>S \<alpha>. (S
   by (metis Un_iff case_prod_conv in_set_conv_decomp insertCI nt.simps(2) nt_append)
 
 lemma slemma4_4:
-  assumes "trans1Tmnl A t P P'"
+  assumes "trans1Tm A t P P'"
     and "(l,r) \<in> set P"
   shows "(Nt A) \<notin> set r"
 proof -
   have "A \<notin> nts (set P)"
-    using assms(1) unfolding trans1Tmnl_def by blast
+    using assms(1) fresh unfolding trans1Tm_def by blast
   hence "\<nexists>S \<alpha>. (S, \<alpha>) \<in> set P \<and> (Nt A \<in> {Nt S} \<union> set \<alpha>)"
     using nts_correct[of A \<open>set P\<close>] by blast
   thus ?thesis 
@@ -288,7 +282,7 @@ lemma slemma4_4Nt:
   shows "(Nt A) \<notin> set r"
 proof -
   have "A \<notin> nts (set P)"
-    using assms(1) unfolding trans2Nt_def by blast
+    using assms(1) fresh unfolding trans2Nt_def by blast
   hence "\<nexists>S \<alpha>. (S, \<alpha>) \<in> set P \<and> (Nt A \<in> {Nt S} \<union> set \<alpha>)"
     using nts_correct[of A \<open>set P\<close>] by blast
   thus ?thesis 
@@ -297,13 +291,13 @@ qed
 
 
 lemma lemma1:
-  assumes "trans1Tmnl A t P P'"
+  assumes "trans1Tm A t P P'"
     and "set P' \<turnstile> lhs \<Rightarrow> rhs"
   shows "(elim (A, [Tm t]) lhs = elim (A, [Tm t]) rhs) \<or> (set P \<turnstile> (elim (A, [Tm t]) lhs) \<Rightarrow> (elim (A, [Tm t]) rhs))"
 proof -
   obtain l r p s where "(l,r) \<in> set P \<and> (r = p@[Tm t]@s) \<and> (p \<noteq> [] \<or> s \<noteq> []) \<and> (A \<notin> nts (set P)) 
       \<and> set P' = ((set P - {(l,r)}) \<union> {(A,[Tm t]), (l, p@[Nt A]@s)})" (is "?lrps")
-    using assms(1) set_removeAll unfolding trans1Tmnl_def by force
+    using assms(1) set_removeAll fresh unfolding trans1Tm_def by fastforce
   obtain p' s' u v where "lhs = p'@[Nt u]@s' \<and> rhs = p'@v@s' \<and> (u,v) \<in> set P'" (is "?uv")
     using assms(2) derive.cases by meson
   thus ?thesis
@@ -374,7 +368,7 @@ lemma lemma1Nt:
 proof -
   obtain l r p s where "(l,r) \<in> set P \<and> (r = p@[Nt B\<^sub>1,Nt B\<^sub>2]@s) \<and> (p \<noteq> [] \<or> s \<noteq> []) \<and> (A \<notin> nts (set P))
     \<and> (set P' = ((set P - {(l,r)}) \<union> {(A, [Nt B\<^sub>1,Nt B\<^sub>2]), (l, p@[Nt A]@s)}))" (is "?lrps")
-    using assms(1) set_removeAll unfolding trans2Nt_def by force
+    using assms(1) set_removeAll fresh unfolding trans2Nt_def by fastforce
   obtain p' s' u v where "lhs = p'@[Nt u]@s' \<and> rhs = p'@v@s' \<and> (u,v) \<in> set P'" (is "?uv")
     using assms(2) derive.cases by meson
   thus ?thesis
@@ -445,7 +439,7 @@ qed
 
 lemma lemma3:
   assumes "set P' \<turnstile> lhs \<Rightarrow>* rhs"
-    and "trans1Tmnl A t P P'"
+    and "trans1Tm A t P P'"
   shows "set P \<turnstile> (elim (A, [Tm t]) lhs) \<Rightarrow>* (elim (A, [Tm t]) rhs)"
   using assms
 proof (induction)
@@ -469,19 +463,19 @@ lemma slemma4_7: "map Tm w = elim (A, \<alpha>) (map Tm w)"
   by (induction w) auto
 
 lemma slemma4_2: 
-  assumes "trans1Tmnl A t P P'"
+  assumes "trans1Tm A t P P'"
     and "N \<in> nts (set P)"
   shows "[Nt N] = elim (A, [Tm t]) [Nt N]"
-  using assms unfolding trans1Tmnl_def by auto
+  using assms fresh unfolding trans1Tm_def by auto
 
 lemma slemma4_2Nt: 
   assumes "trans2Nt A B\<^sub>1 B\<^sub>2 P P'"
     and "N \<in> nts (set P)"
   shows "[Nt N] = elim (A, [Nt B\<^sub>1, Nt B\<^sub>2]) [Nt N]"
-  using assms unfolding trans2Nt_def by auto
+  using assms fresh unfolding trans2Nt_def by auto
 
 lemma lemma4:
-  assumes "trans1Tmnl A t P P'" 
+  assumes "trans1Tm A t P P'" 
     and "S \<in> nts (set P)"
   shows "lang P' S \<subseteq> lang P S"
 proof 
@@ -490,11 +484,11 @@ proof
   hence "set P' \<turnstile> [Nt S] \<Rightarrow>* map Tm w"
     unfolding Lang_def by simp
   hence "set P' \<turnstile> [Nt S] \<Rightarrow>* map Tm w"
-    using assms unfolding trans1Tmnl_def by auto
+    using assms unfolding trans1Tm_def by auto
   hence "set P \<turnstile> elim (A, [Tm t]) [Nt S] \<Rightarrow>*  elim (A, [Tm t]) (map Tm w)"
     using assms lemma3[of P' \<open>[Nt S]\<close> \<open>map Tm w\<close> A t P] by blast
   moreover have "elim (A, [Tm t]) [Nt S] = [Nt S]"
-    using assms unfolding trans1Tmnl_def by auto
+    using assms fresh unfolding trans1Tm_def by auto
   moreover have "elim (A, [Tm t]) (map Tm w) = map Tm w" 
     using \<open>w \<in> lang P' S\<close> slemma4_7 by metis
   ultimately show "w \<in> lang P S" 
@@ -515,7 +509,7 @@ proof
   hence "set P \<turnstile> elim (A, [Nt B\<^sub>1, Nt B\<^sub>2]) [Nt S] \<Rightarrow>*  elim (A, [Nt B\<^sub>1, Nt B\<^sub>2]) (map Tm w)"
     using assms lemma3Nt[of P' \<open>[Nt S]\<close> \<open>map Tm w\<close> A B\<^sub>1 B\<^sub>2 P] by blast
   moreover have "elim (A, [Nt B\<^sub>1, Nt B\<^sub>2]) [Nt S] = [Nt S]"
-    using assms unfolding trans2Nt_def by auto 
+    using assms fresh unfolding trans2Nt_def by auto 
   moreover have "elim (A, [Nt B\<^sub>1, Nt B\<^sub>2]) (map Tm w) = map Tm w" 
     using \<open>w \<in> lang P' S\<close> slemma4_7 by metis
   ultimately show "w \<in> lang P S" using Lang_def \<open>w \<in> lang P' S\<close> 
@@ -525,7 +519,7 @@ qed
 lemma slemma5_1:
   assumes "set P \<turnstile> lhs \<Rightarrow>* rhs"
     and "lhs = [Nt S]"
-    and "trans1Tmnl A t P P'"
+    and "trans1Tm A t P P'"
   shows "set P' \<turnstile> lhs \<Rightarrow>* rhs"
   using assms apply (induction) apply auto by (meson cnf_r1Tm rtranclp_trans)
 
@@ -537,7 +531,7 @@ lemma slemma5_1Nt:
   using assms apply (induction) apply auto by (meson cnf_r1Nt rtranclp_trans)
 
 lemma lemma5: 
-  assumes "trans1Tmnl A t P P'"
+  assumes "trans1Tm A t P P'"
   shows "lang P S \<subseteq> lang P' S"
 proof 
   fix w
@@ -561,7 +555,7 @@ proof
 qed 
 
 lemma cnf_lemma1: 
-  assumes "trans1Tmnl A t P P'" "S \<in> nts (set P)"
+  assumes "trans1Tm A t P P'" "S \<in> nts (set P)"
   shows "lang P S = lang P' S"
   using assms lemma4 lemma5 by fast
 
@@ -573,11 +567,11 @@ lemma cnf_lemma1Nt:
 definition eqLang :: "('n,'t) prods \<Rightarrow> ('n,'t) prods \<Rightarrow> 'n \<Rightarrow> bool" where
   "eqLang P P' S \<longleftrightarrow> lang P S = lang P' S"
 
-lemma trans1TmnlRtc_noeProds: 
-  assumes "((\<lambda>x y. \<exists>A t. trans1Tmnl A t x y) ^**) P P'"
+lemma trans1TmRtc_noeProds: 
+  assumes "((\<lambda>x y. \<exists>A t. trans1Tm A t x y) ^**) P P'"
     and "noeProds (set P)"
   shows "noeProds (set P')"
-  using assms by (induction) (auto simp: trans1Tmnl_noeProds)
+  using assms by (induction) (auto simp: trans1Tm_noeProds)
 
 lemma trans2NtRtc_noeProds:
   assumes "((\<lambda>x y. \<exists>A t B\<^sub>1 B\<^sub>2. trans2Nt A B\<^sub>1 B\<^sub>2 x y) ^**) P P'"
@@ -585,11 +579,11 @@ lemma trans2NtRtc_noeProds:
   shows "noeProds (set P')"
   using assms by (induction) (auto simp: trans2Nt_noeProds)
 
-lemma trans1TmnlRtc_noUnitProds: 
-  assumes "((\<lambda>x y. \<exists>A t. trans1Tmnl A t x y) ^**) P P'"
+lemma trans1TmRtc_noUnitProds: 
+  assumes "((\<lambda>x y. \<exists>A t. trans1Tm A t x y) ^**) P P'"
     and "noUnitProds (set P)"
   shows "noUnitProds (set P')"
-  using assms by (induction) (auto simp: trans1Tmnl_noUnitProds)
+  using assms by (induction) (auto simp: trans1Tm_noUnitProds)
 
 lemma trans2NtRtc_noUnitProds:
   assumes "((\<lambda>x y. \<exists>A t B\<^sub>1 B\<^sub>2. trans2Nt A B\<^sub>1 B\<^sub>2 x y) ^**) P P'"
@@ -602,13 +596,13 @@ lemma trans2NtRtc_noUnitProds:
 lemma nts_aux1: "nts (P \<union> P') = nts P \<union> nts P'"
   unfolding nts_def by simp
 
-lemma trans1Tmnl_nts: 
-  assumes "trans1Tmnl A t P P'" "S \<in> nts (set P)"
+lemma trans1Tm_nts: 
+  assumes "trans1Tm A t P P'" "S \<in> nts (set P)"
   shows "S \<in> nts (set P')"
 proof -
   obtain l r p s where "(l,r) \<in> set P \<and> (r = p@[Tm t]@s) \<and> (p \<noteq> [] \<or> s \<noteq> []) \<and> (A \<notin> nts (set P)) 
       \<and> set P' = ((set P - {(l,r)}) \<union> {(A,[Tm t]), (l, p@[Nt A]@s)})" (is "?lrps")
-    using assms(1) set_removeAll unfolding trans1Tmnl_def by force
+    using assms(1) set_removeAll fresh unfolding trans1Tm_def by fastforce
   thus ?thesis
   proof (cases "S \<in> nts {(l,r)}")
     case True
@@ -625,10 +619,10 @@ proof -
   qed
 qed  
 
-lemma trans1TmnlRtc_nts: 
-  assumes "((\<lambda>x y. \<exists>A t. trans1Tmnl A t x y) ^**) P P'" "S \<in> nts (set P)"
+lemma trans1TmRtc_nts: 
+  assumes "((\<lambda>x y. \<exists>A t. trans1Tm A t x y) ^**) P P'" "S \<in> nts (set P)"
   shows "S \<in> nts (set P')"
-  using assms by (induction rule: rtranclp.induct) (auto simp: trans1Tmnl_nts)
+  using assms by (induction rule: rtranclp.induct) (auto simp: trans1Tm_nts)
 
 lemma trans2Nt_nts: 
   assumes "trans2Nt A B\<^sub>1 B\<^sub>2 P P'" "S \<in> nts (set P)"
@@ -636,7 +630,7 @@ lemma trans2Nt_nts:
 proof -
   obtain l r p s where "(l,r) \<in> set P \<and> (r = p@[Nt B\<^sub>1,Nt B\<^sub>2]@s) \<and> (p \<noteq> [] \<or> s \<noteq> []) \<and> (A \<notin> nts (set P))
     \<and> (set P' = ((set P - {(l,r)}) \<union> {(A, [Nt B\<^sub>1,Nt B\<^sub>2]), (l, p@[Nt A]@s)}))" (is "?lrps")
-    using assms(1) set_removeAll unfolding trans2Nt_def by force
+    using assms(1) set_removeAll fresh unfolding trans2Nt_def by fastforce
     thus ?thesis
   proof (cases "S \<in> nts {(l,r)}")
     case True
@@ -662,9 +656,9 @@ lemma trans2NtRtc_nts:
 (* Termination for an arbitrary start Symbol S *)
 
 theorem cnf_lemma2: 
-  assumes "((\<lambda>x y. \<exists>A t. trans1Tmnl A t x y) ^**) P P'" "S \<in> nts (set P)" 
+  assumes "((\<lambda>x y. \<exists>A t. trans1Tm A t x y) ^**) P P'" "S \<in> nts (set P)" 
   shows "(lang P S = lang P' S)"
-  using assms by (induction rule: rtranclp.induct) (fastforce simp: cnf_lemma1 trans1TmnlRtc_nts)+
+  using assms by (induction rule: rtranclp.induct) (fastforce simp: cnf_lemma1 trans1TmRtc_nts)+
 
 theorem cnf_lemma2Nt: 
   assumes "((\<lambda>x y. \<exists>A B\<^sub>1 B\<^sub>2. trans2Nt A B\<^sub>1 B\<^sub>2 x y) ^**) P P'" "S \<in> nts (set P)" 
@@ -672,11 +666,11 @@ theorem cnf_lemma2Nt:
   using assms by (induction rule: rtranclp.induct) (fastforce simp: cnf_lemma1Nt trans2NtRtc_nts)+
 
 theorem cnf_lemma: 
-  assumes "((\<lambda>x y. \<exists>A t. trans1Tmnl A t x y) ^**) P P'"
+  assumes "((\<lambda>x y. \<exists>A t. trans1Tm A t x y) ^**) P P'"
     and "((\<lambda>x y. \<exists>A B\<^sub>1 B\<^sub>2. trans2Nt A B\<^sub>1 B\<^sub>2 x y) ^**) P' P''"
     and "S \<in> nts (set P)"
   shows "lang P S = lang P'' S"
-  using assms cnf_lemma2 cnf_lemma2Nt trans1TmnlRtc_nts by fastforce
+  using assms cnf_lemma2 cnf_lemma2Nt trans1TmRtc_nts by fastforce
 
 (* Part 2 *)
 lemma badTmsCount_append: "badTmsCount (P@P') = badTmsCount P + badTmsCount P'"
@@ -695,18 +689,23 @@ lemma badNtsCount_removeAll:
   shows "badNtsCount (removeAll p P) < badNtsCount P"
   using assms by (induction P) fastforce+
 
-lemma badTmnsCount_removeAll2:
+lemma badTmsCount_removeAll2:
   assumes "prodTms p > 0" "p \<in> set P" "prodTms p' < prodTms p"
   shows "badTmsCount (removeAll p P) + prodTms p' < badTmsCount P"
   using assms by (induction P) fastforce+
 
+lemma badNtsCount_removeAll2:
+  assumes "prodNts p > 0" "p \<in> set P" "prodNts p' < prodNts p"
+  shows "badNtsCount (removeAll p P) + prodNts p' < badNtsCount P"
+  using assms by (induction P) fastforce+
+
 lemma lemma6_a: 
-  assumes "trans1Tmnl A t P P'" 
+  assumes "trans1Tm A t P P'" 
   shows "badTmsCount P' < badTmsCount P"
 proof -
   obtain l r p s where "(l,r) \<in> set P \<and> (r = p@[Tm t]@s) \<and> (p \<noteq> [] \<or> s \<noteq> []) \<and> (A \<notin> nts (set P)) 
       \<and> P' = ((removeAll (l,r) P) @ [(A,[Tm t]), (l, p@[Nt A]@s)])" (is "?lrps")
-    using assms unfolding trans1Tmnl_def by auto
+    using assms fresh unfolding trans1Tm_def by auto
   hence "prodTms (l,p@[Tm t]@s) = length (filter (isTmnlSym) (p@[Tm t]@s))"
     unfolding prodTms_def by auto
   hence 1: "prodTms (l,p@[Tm t]@s) = Suc (length (filter (isTmnlSym) (p@s)))"
@@ -725,7 +724,7 @@ proof -
     moreover have "prodTms (l,p@[Nt A]@s) < prodTms (l,p@[Tm t]@s)"
       using 1 \<open>prodTms (l, p @ [Nt A] @ s) = length (filter isTmnlSym (p @ [Nt A] @ s))\<close> isTmnlSym_def by force 
     ultimately show "badTmsCount P' < badTmsCount P" 
-      using badTmnsCount_removeAll2[of "(l,r)" P "(l,p @[Nt A]@s)"] \<open>?lrps\<close> 1 by auto
+      using badTmsCount_removeAll2[of "(l,r)" P "(l,p @[Nt A]@s)"] \<open>?lrps\<close> 1 by auto
   next 
     assume "prodTms (l, p@[Nt A]@s) = 0"
     hence "badTmsCount P' = badTmsCount (removeAll (l,r) P)"
@@ -735,13 +734,13 @@ proof -
   qed
 qed
 
-lemma slemma6_b: 
+lemma lemma6_b: 
   assumes "trans2Nt A B\<^sub>1 B\<^sub>2 P P'"
   shows "badNtsCount P' < badNtsCount P"
 proof -
   obtain l r p s where "(l,r) \<in> set P \<and> (r = p@[Nt B\<^sub>1,Nt B\<^sub>2]@s) \<and> (p \<noteq> [] \<or> s \<noteq> []) \<and> (A \<notin> nts (set P))
     \<and> (P' = ((removeAll (l,r) P) @ [(A, [Nt B\<^sub>1,Nt B\<^sub>2]), (l, p@[Nt A]@s)]))" (is "?lrps")
-    using assms(1) unfolding trans2Nt_def by auto
+    using assms(1) fresh unfolding trans2Nt_def by auto
   hence "prodNts (l,p@[Nt B\<^sub>1,Nt B\<^sub>2]@s) = length (filter (isNonTmnlSym) (p@[Nt B\<^sub>1,Nt B\<^sub>2]@s))"
     unfolding prodNts_def by auto
   hence 1: "prodNts (l,p@[Nt B\<^sub>1,Nt B\<^sub>2]@s) = Suc (Suc (length (filter (isNonTmnlSym) (p@s))))"
@@ -752,14 +751,108 @@ proof -
     using \<open>?lrps\<close> badNtsCount_removeAll 1 by force
   have "prodNts (l, p@[Nt A]@s) = length (filter (isNonTmnlSym) (p@[Nt A]@s)) \<or> prodNts (l, p@[Nt A]@s) = 0"
     unfolding prodNts_def using \<open>?lrps\<close> by simp
-  thus ?thesis sorry
+  thus ?thesis 
+  proof 
+    assume "prodNts (l, p@[Nt A]@s) = length (filter (isNonTmnlSym) (p@[Nt A]@s))"
+    hence "badNtsCount P' = badNtsCount (removeAll (l,r) P) + badNtsCount [(l, (p@[Nt A]@s))]"
+      using 2 by (simp add: prodNts_def)
+    moreover have "prodNts (l, p@[Nt A]@s) < prodNts (l,p@[Nt B\<^sub>1,Nt B\<^sub>2]@s)"
+      using 1 \<open>prodNts (l, p@[Nt A]@s) = length (filter (isNonTmnlSym) (p@[Nt A]@s))\<close> isNonTmnlSym_def by simp
+    ultimately show ?thesis 
+      using badNtsCount_removeAll2[of "(l,r)" P "(l, (p@[Nt A]@s))"] 1 \<open>?lrps\<close> by auto
+  next 
+    assume "prodNts (l, p@[Nt A]@s) = 0"
+    hence "badNtsCount P' = badNtsCount (removeAll (l,r) P)"
+      using 2 by (simp add: prodNts_def)
+    thus ?thesis 
+      using 3 by simp
+  qed
 qed
 
+lemma lemma7_a: "trans1Tm A t P P' \<Longrightarrow> badTmsCount P > 0"
+  using lemma6_a by fastforce
 
+lemma lemma7_b: "trans2Nt A B\<^sub>1 B\<^sub>2 P P' \<Longrightarrow> badNtsCount P > 0"
+  using lemma6_b by fastforce
 
-theorem trans1Tmnl_2: 
-  assumes "infinite(UNIV::'a set)"
-  shows "\<exists>P'. ((\<lambda>x y. \<exists>A t. trans1Tmnl A t x y) ^**) P P' \<and> (badTms (set P'))"
+lemma badTmsCount0_removeAll: "badTmsCount P = 0 \<Longrightarrow> badTmsCount (removeAll (l,r) P) = 0" 
+  by (induction P) auto 
+
+lemma slemma15_a:
+  assumes "trans2Nt A B\<^sub>1 B\<^sub>2 P P'"
+    and "badTmsCount P = 0"
+  shows "badTmsCount P' = 0"
+proof -
+  obtain l r p s where "(l,r) \<in> set P \<and> (r = p@[Nt B\<^sub>1,Nt B\<^sub>2]@s) \<and> (p \<noteq> [] \<or> s \<noteq> []) \<and> (A \<notin> nts (set P))
+    \<and> (P' = ((removeAll (l,r) P) @ [(A, [Nt B\<^sub>1,Nt B\<^sub>2]), (l, p@[Nt A]@s)]))" (is "?lrps")
+    using assms(1) fresh unfolding trans2Nt_def by auto
+  hence "badTmsCount P' = badTmsCount (removeAll (l,r) P) + badTmsCount [(l, (p@[Nt A]@s))]"
+    by (auto simp: badTmsCount_append prodTms_def isTmnlSym_def)
+  moreover have "badTmsCount (removeAll (l,r) P) = 0"
+    using badTmsCount0_removeAll[of P l r] assms(2) by simp
+  moreover have "badTmsCount [(l, (p@[Nt A]@s))] = 0" 
+  proof -
+    have "prodTms (l,p@[Nt B\<^sub>1,Nt B\<^sub>2]@s) = 0"
+      using \<open>?lrps\<close> assms(2) badTmsCountSet by auto
+    thus "badTmsCount [(l, (p@[Nt A]@s))] = 0"
+      by (auto simp: isTmnlSym_def prodTms_def)
+  qed
+  ultimately show ?thesis 
+    by simp
+qed
+
+lemma lemma15_a:
+  assumes "((\<lambda>x y. \<exists>A B\<^sub>1 B\<^sub>2. trans2Nt A B\<^sub>1 B\<^sub>2 x y) ^**) P P'"
+    and "badTmsCount P = 0"
+  shows "badTmsCount P' = 0"
+  using assms by (induction) (auto simp: slemma15_a)
+
+lemma noTms_prodTms0:
+  assumes "prodTms (l,r) = 0"
+  shows "length r \<le> 1 \<or> (\<forall>a \<in> set r. isNonTmnlSym a)"
+proof -
+  have "length r \<le> 1 \<or> (\<nexists>a. a \<in> set r \<and> isTmnlSym a)"
+    using assms unfolding prodTms_def using empty_filter_conv by fastforce
+  thus ?thesis 
+    by (metis isNonTmnlSym_def isTmnlSym_def sym.exhaust)
+qed
+
+lemma list_longer3: "length l \<ge> 3 \<Longrightarrow> (\<exists>hd tl x y. l = hd@[x]@[y]@tl \<and> (hd \<noteq> [] \<or> tl \<noteq> []))"
+  by (metis Suc_le_length_iff append.left_neutral append_Cons neq_Nil_conv numeral_3_eq_3)
+
+lemma badNtsCountNot0: 
+  assumes "badNtsCount P > 0" 
+  shows "(\<exists>l r. (l, r) \<in> set P \<and> length r \<ge> 3)"
+proof -
+  have "\<exists>p \<in> set P. prodNts p > 0"
+    using assms badNtsCountSet not_gr0 by blast
+  from this obtain l r where "(l, r) \<in> set P \<and> prodNts (l,r) > 0" (is "?lr")
+    by auto
+  hence "length r \<ge> 3"
+    unfolding prodNts_def using not_le_imp_less by fastforce
+  thus ?thesis using \<open>?lr\<close> by auto
+qed
+
+lemma lemma8_b:
+  assumes "badTmsCount P = 0"
+    and "badNtsCount P > 0"
+  shows "\<exists>P' A B\<^sub>1 B\<^sub>2. trans2Nt A B\<^sub>1 B\<^sub>2 P P'"
+proof -
+  obtain l r where "(l, r) \<in> set P \<and> length r \<ge> 3" (is "?lr")
+    using assms(2) badNtsCountNot0 by blast
+  obtain p s X Y where "r = p@[X]@[Y]@s \<and> (p \<noteq> [] \<or> s \<noteq> [])" (is "?psXY")
+    using \<open>?lr\<close> list_longer3[of r] by blast
+  have "(\<forall>a \<in> set r. isNonTmnlSym a)"
+    using \<open>?lr\<close> assms(1) badTmsCountSet[of P] noTms_prodTms0[of l r] by simp
+  hence "\<exists>B\<^sub>1 B\<^sub>2. X = Nt B\<^sub>1 \<and> Y = Nt B\<^sub>2"
+    using isNonTmnlSym_def \<open>?psXY\<close> by auto
+  hence "\<exists>B\<^sub>1 B\<^sub>2. (r = p@[Nt B\<^sub>1,Nt B\<^sub>2]@s) \<and> (p \<noteq> [] \<or> s \<noteq> [])"
+    using \<open>?psXY\<close> by auto
+  thus ?thesis
+    using trans2Nt_def \<open>?lr\<close> by blast
+qed
+
+theorem trans1Tm_2: "\<exists>P'. ((\<lambda>x y. \<exists>A t. trans1Tm A t x y) ^**) P P' \<and> (badTmsCount P' = 0)"
   sorry
 
 definition "isCnf P \<equiv> (\<forall>l r. (l,r) \<in> set P \<longrightarrow> (
